LinearScan/ssrbool.hs
@@ -1,8 +1,22 @@
+{-# OPTIONS_GHC -cpp -fglasgow-exts #-}
+{- For Hugs, use the option -F"cpp -P -traditional" -}
+
 module LinearScan.Ssrbool where
 
 import qualified Prelude
 import qualified Data.List
 import qualified LinearScan.Utils
+
+
+--unsafeCoerce :: a -> b
+#ifdef __GLASGOW_HASKELL__
+import qualified GHC.Base as GHC.Base
+unsafeCoerce = GHC.Base.unsafeCoerce#
+#else
+-- HUGS
+import qualified LinearScan.IOExts as IOExts
+unsafeCoerce = IOExts.unsafeCoerce
+#endif
 
 __ :: any
 __ = Prelude.error "Logical or arity value used"
@@ -28,4 +42,30 @@ idP b1 =
 type Coq_pred t = t -> Prelude.Bool
 
 type Coq_rel t = t -> Coq_pred t
+
+data Coq_mem_pred t =
+   Mem (Coq_pred t)
+
+data Coq_predType t =
+   PredType (() -> Coq_pred t) (() -> Coq_mem_pred t)
+
+type Coq_pred_sort t = ()
+
+mkPredType :: (a2 -> a1 -> Prelude.Bool) -> Coq_predType a1
+mkPredType toP =
+  PredType (unsafeCoerce toP) (\p -> Mem (\x -> unsafeCoerce toP p x))
+
+pred_of_mem :: (Coq_mem_pred a1) -> Coq_pred_sort a1
+pred_of_mem mp =
+  case mp of {
+   Mem p -> unsafeCoerce (\x -> p x)}
+
+mem :: (Coq_predType a1) -> (Coq_pred_sort a1) -> Coq_mem_pred a1
+mem pT =
+  case pT of {
+   PredType topred s -> s}
+
+in_mem :: a1 -> (Coq_mem_pred a1) -> Prelude.Bool
+in_mem x mp =
+  unsafeCoerce (\_ -> pred_of_mem) __ mp x
 
